thy/Routing/LinuxRouter.thy
@@ -1,14 +1,20 @@
 theory LinuxRouter
-imports Routing "../Simple_Firewall/SimpleFw_Semantics"
+imports 
+	(* For obvious reasons *)
+	Routing
+	"../Simple_Firewall/SimpleFw_Semantics"
+	(* for the simple packet extension *)
+	"../OpenFlow/OpenFlowMatches"
 begin
-
-term "map port_sel $ routing_table_semantics rt (p_dst p)"
+definition "fromMaybe a m = (case m of Some a \<Rightarrow> a | None \<Rightarrow> a)" (* mehr Haskell wagen *)
+term "routing_table_semantics rt (p_dst p)"
 definition "simple_linux_router rt fw p \<equiv> let
 	rd = routing_table_semantics rt (p_dst p) in
 	concat (map (\<lambda>pt. case (simple_fw fw (p_oiface_update (const (port_sel pt)) p)) of 
 		Decision FinalAllow \<Rightarrow> [pt] |
 		Decision FinalDeny \<Rightarrow> []
 	) rd)"
-(* Todo: Find something that looks a bit more semantic *)
+(* Todo: Find something that looks a bit more semantic. And update source and destination macs *)
+term p_l2dst_update
 
 end
